theories/Algorithmic/Typing/Definitions.v
@@ -6,82 +6,103 @@ From McPTS.Core.Syntactic Require Export SystemOpt.
 Import Syntax_Notations.
 
 
-Reserved Notation "⟪ pred_P ⟫ Γ '⊢a' M ⟹ A" (in custom judg at level 80, pred_P constr, Γ custom exp, M custom exp, A custom nf).
-Reserved Notation "⟪ pred_P ⟫ Γ '⊢a' M ⟸ A" (in custom judg at level 80, pred_P constr, Γ custom exp, M custom exp, A custom exp).
+Reserved Notation "Γ '⊢a' M ⟹ A" (in custom judg at level 80, Γ custom exp, M custom exp, A custom nf).
+Reserved Notation "Γ '⊢a' M ⟸ A" (in custom judg at level 80, Γ custom exp, M custom exp, A custom exp).
+Reserved Notation "Γ '⊢as' σ ⟹ Δ" (in custom judg at level 80, Γ custom exp, σ custom exp, Δ custom exp).
+Reserved Notation "Γ '⊢as' σ ⟸ Δ" (in custom judg at level 80, Γ custom exp, σ custom exp, Δ custom exp).
 
 Generalizable All Variables.
 
-(* Record ConvertibleSig (P : PtsSig) : Type := *)
-(*   mkConvertibleSig { *)
-(*       Convert : ctx P -> typ P -> typ P -> Prop; *)
-(*       CorrectConv : forall Γ A B, Convert Γ A B <-> {{ Γ ⊢ A ⊆ B }}; *)
-(*       DecidableConv : forall Γ A B, (Convert Γ A B) \/ ~(Convert Γ A B); *)
-(*     }. *)
-(* Arguments Convert {_}. *)
-(* Arguments CorrectConv {_}. *)
-(* Arguments DecidableConv {_}. *)
-
-Inductive alg_type_check {P} (pred_P : PredicativeSig P) : ctx P -> typ P -> exp P -> Prop :=             
+Inductive alg_type_check {P} : ctx P -> typ P -> exp P -> Prop :=             
 (** Conversion *)
-| atc_conv : `( {{ ⟪ pred_P ⟫ Γ ⊢a M ⟹ A }} ->
+| atc_conv : `( {{ Γ ⊢a M ⟹ A }} ->
                 {{ Γ ⊢a A ⊆ B }} ->
-                {{ ⟪ pred_P ⟫ Γ ⊢a M ⟸ B }} )
+                {{ Γ ⊢a M ⟸ B }} )
               
-where "⟪ pred_P ⟫ Γ '⊢a' M ⟸ A" := (alg_type_check pred_P Γ A M) (in custom judg) : type_scope
+where "Γ '⊢a' M ⟸ A" := (alg_type_check Γ A M) (in custom judg) : type_scope
 
-with alg_type_infer {P} (pred_P : PredicativeSig P) : ctx P -> nf P -> exp P -> Prop :=
+with alg_type_infer {P} : ctx P -> nf P -> exp P -> Prop :=
 (** Variables *)
 | ati_var : `( {{ #x : A @ s ∈ Γ }} ->
                nbe_ty Γ A B ->
-               {{ ⟪ pred_P ⟫ Γ ⊢a #x ⟹ B }} )
+               {{ Γ ⊢a #x ⟹ B }} )
 
 (** Sorts *)
 | ati_st : `( Ax_typ P s1 s2 ->
-              {{ ⟪ pred_P ⟫  Γ ⊢a Sort@s1 ⟹ Sort@s2 }} )
+              {{ Γ ⊢a Sort@s1 ⟹ Sort@s2 }} )
              
 (** Functions *)
 | atc_pi : `( forall {r : Ru_pi P s1 s2 s3},
-                 {{ ⟪ pred_P ⟫  Γ ⊢a A ⟸ Sort@s1 }} ->
-                 {{ ⟪ pred_P ⟫  Γ, A@s1 ⊢a B ⟸ Sort@s2 }} ->
-                 {{ ⟪ pred_P ⟫  Γ ⊢a Π r A B ⟹ Sort@s3 }} )
+                 {{ Γ ⊢a A ⟸ Sort@s1 }} ->
+                 {{ Γ, A@s1 ⊢a B ⟸ Sort@s2 }} ->
+                 {{ Γ ⊢a Π r A B ⟹ Sort@s3 }} )
 
 | ati_lam : `( forall {r : Ru_pi P s1 s2 s3},
-                  {{ ⟪ pred_P ⟫ Γ ⊢a A ⟸ Sort@s1 }} ->
-                  {{ ⟪ pred_P ⟫ Γ, A@s1 ⊢a B ⟸ Sort@s2 }} ->
-                  {{ ⟪ pred_P ⟫ Γ, A@s1 ⊢a M ⟹ D }} ->
+                  {{ Γ ⊢a A ⟸ Sort@s1 }} ->
+                  {{ Γ, A@s1 ⊢a B ⟸ Sort@s2 }} ->
+                  {{ Γ, A@s1 ⊢a M ⟹ D }} ->
                   nbe {{{ Γ, A@s1 }}} B {{{ Sort@s2 }}} D ->
                   nbe Γ A {{{ Sort@s1 }}} C ->
-                  {{ ⟪ pred_P ⟫ Γ ⊢a λ r A M ⟹ Π r C D }} )
+                  {{ Γ ⊢a λ r A M ⟹ Π r C D }} )
              
 | ati_app : `( forall {r : Ru_pi P s1 s2 s3},
-                  {{ ⟪ pred_P ⟫ Γ ⊢a M ⟹ Π r A B }} ->
-                  {{ ⟪ pred_P ⟫ Γ ⊢a N ⟸ A }} ->
+                  {{ Γ ⊢a M ⟹ Π r A B }} ->
+                  {{ Γ ⊢a N ⟸ A }} ->
                   nbe_ty Γ {{{ B[Id,,N] }}} C ->
-                  {{ ⟪ pred_P ⟫ Γ ⊢a M N ⟹ C }} )
+                  {{ Γ ⊢a M N ⟹ C }} )
                   
 (** Naturals *)
 | ati_nat : `( Ru_nat P s ->
-               {{ ⟪ pred_P ⟫ Γ ⊢a ℕ ⟹ Sort@s }} )
+               {{ Γ ⊢a ℕ ⟹ Sort@s }} )
 | ati_zero : `( Ru_nat P s ->
-                {{ ⟪ pred_P ⟫ Γ ⊢a zero ⟹ ℕ }} )
+                {{ Γ ⊢a zero ⟹ ℕ }} )
 | ati_succ : `( Ru_nat P s ->
-                {{ ⟪ pred_P ⟫ Γ ⊢a M ⟸ ℕ }} ->
-                {{ ⟪ pred_P ⟫ Γ ⊢a succ M ⟹ ℕ }} )
+                {{ Γ ⊢a M ⟸ ℕ }} ->
+                {{ Γ ⊢a succ M ⟹ ℕ }} )
 | ati_rec : `( Ru_nat P s ->
-               {{ ⟪ pred_P ⟫ Γ, ℕ@s ⊢a A ⟹ Sort@s' }} ->
-               {{ ⟪ pred_P ⟫ Γ ⊢a MZ ⟸ A[Id,,zero] }} ->
-               {{ ⟪ pred_P ⟫ Γ, ℕ@s, A@s' ⊢a MS ⟸ A[Wk∘Wk,,succ #1] }} ->
-               {{ ⟪ pred_P ⟫ Γ ⊢a N ⟸ ℕ }} ->
+               {{ Γ, ℕ@s ⊢a A ⟹ Sort@s' }} ->
+               {{ Γ ⊢a MZ ⟸ A[Id,,zero] }} ->
+               {{ Γ, ℕ@s, A@s' ⊢a MS ⟸ A[Wk∘Wk,,succ #1] }} ->
+               {{ Γ ⊢a N ⟸ ℕ }} ->
                nbe_ty Γ {{{ A[Id,,N] }}} B ->
-               {{ ⟪ pred_P ⟫ Γ ⊢a rec N return A | zero -> MZ | succ -> MS end ⟹ B }} )
-where "⟪ pred_P ⟫ Γ '⊢a' M ⟹ A" := (alg_type_infer pred_P Γ A M) (in custom judg) : type_scope.
+               {{ Γ ⊢a rec N return A | zero -> MZ | succ -> MS end ⟹ B }} )
+
+(** Explicit substitutions *)
+| ati_clo : `( {{ Γ ⊢as σ ⟹ Δ }} ->
+               {{ Δ ⊢a M ⟹ A }} ->
+               nbe_ty Γ {{{ A[σ] }}} W ->
+               {{ Γ ⊢a M[σ] ⟹ W }} )
+where "Γ '⊢a' M ⟹ A" := (alg_type_infer Γ A M) (in custom judg) : type_scope
+
+with alg_type_check_sub {P} : ctx P -> ctx P -> sub P -> Prop :=
+| atc_sub : `( {{ Γ ⊢as σ ⟹ Δ }} ->
+               {{ ⊢a Δ ⊆ Δ' }} ->
+               {{ Γ ⊢as σ ⟸ Δ' }} )
+where "Γ ⊢as σ ⟸ Δ" := (alg_type_check_sub Γ Δ σ) (in custom judg) : type_scope
+
+with alg_type_infer_sub {P} : ctx P -> ctx P -> sub P -> Prop :=
+| ati_sub_id : `( {{ Γ ⊢as Id ⟹ Γ }} )
+| ati_sub_weaken : `( {{ Γ, A@s ⊢as Wk ⟹ Γ }} )
+| ati_sub_compose : `( {{ Γ1 ⊢as σ2 ⟹ Γ2 }} ->
+                       {{ Γ2 ⊢as σ1 ⟹ Γ3 }} ->
+                       {{ Γ1 ⊢as σ1∘σ2 ⟹ Γ3 }} )
+| ati_sub_extend : `( {{ Γ ⊢as σ ⟹ Δ }} ->
+                      {{ Γ ⊢a M ⟹ A }} ->
+                      {{ Γ ⊢a A ⟹ Sort@s }} ->
+                      {{ Γ ⊢as σ,,M ⟹ Δ, ^(nf_to_exp A)@s }} )
+where "Γ ⊢as σ ⟹ Δ" := (alg_type_infer_sub Γ Δ σ) (in custom judg) : type_scope.
+
 
 
 #[export]
 Hint Constructors alg_type_check alg_type_infer : mcpts.
 
 Scheme alg_type_check_mut_ind := Induction for alg_type_check Sort Prop
-with alg_type_infer_mut_ind := Induction for alg_type_infer Sort Prop.
+with alg_type_infer_mut_ind := Induction for alg_type_infer Sort Prop
+with alg_type_check_sub_mut_ind := Induction for alg_type_check_sub Sort Prop
+with alg_type_infer_sub_mut_ind := Induction for alg_type_infer_sub Sort Prop.
 Combined Scheme alg_type_mut_ind from
   alg_type_check_mut_ind,
-  alg_type_infer_mut_ind.
+  alg_type_infer_mut_ind,
+  alg_type_check_sub_mut_ind,
+  alg_type_infer_sub_mut_ind.
